user 3, session 6414, part 79

diffs-annotated-fixed/3/user-3-session-6414.v
@@ -37,5 +37,100 @@ Module Log (d: OneDiskAPI)<: LogAPI.
 Notation "d [ a |-> b ]" := (diskUpd d a b) (at level 8, left associativity).
 Notation "d [ a |=> bs ]" := (diskUpds d a bs)
   (at level 8, left associativity).
-(* Auto-generated comment: Succeeded. *)
+Opaque diskGet.
+Module Log (d: OneDiskAPI)<: LogAPI.
+Definition len_addr : addr := 0.
+Definition log_addr a : addr := S a.
+Definition init' : proc InitResult :=
+  size <- d.size;
+  (if lt_dec size 1
+   then Ret InitFailed
+   else len0 <- addr_to_block 0; _ <- d.write len_addr len0; Ret Initialized).
+Definition init := then_init d.init init'.
+Definition get_len : proc addr := b <- d.read len_addr; Ret (block_to_addr b).
+Definition get_at (a : addr) : proc block := d.read (log_addr a).
+Fixpoint get_upto (a : addr) : proc (list block) :=
+  match a with
+  | 0 => Ret nil
+  | S a => b <- get_at a; bs <- get_upto a; Ret (bs ++ [b])
+  end.
+Redirect "/var/folders/5x/1mdbpbjd7012l971fq0zkj2w0000gn/T/coqYiLt1m"
+Print Ltac Signatures.
+Timeout 1 Print Grammar tactic.
+Add Search Blacklist "Raw" "Proofs".
+Set Search Output Name Only.
+Redirect "/var/folders/5x/1mdbpbjd7012l971fq0zkj2w0000gn/T/coqy2ao4W"
+SearchPattern _.
+Remove Search Blacklist "Raw" "Proofs".
+Unset Search Output Name Only.
+Definition get : proc (list block) := len <- get_len; get_upto len.
+Fixpoint append_at (a : addr) (bs : list block) : 
+proc unit :=
+  match bs with
+  | [] => Ret tt
+  | b :: bs => _ <- d.write (log_addr a) b; append_at (S a) bs
+  end.
+Definition append (bs : list block) : proc bool :=
+  size <- d.size;
+  len <- get_len;
+  (if le_dec (1 + len + length bs) size
+   then _ <- append_at len bs; Ret true
+   else Ret false).
+Definition reset : proc unit :=
+  len0 <- addr_to_block 0; d.write len_addr len0.
+Definition recover : proc unit := Ret tt.
+Definition log_length_ok (d : disk) (log : list block) :=
+  exists b, diskGet d 0 =?= b /\ block_to_addr b = length log.
+Definition log_abstraction (d : disk) (log : list block) : Prop :=
+  log_length_ok d log /\
+  (forall a, a < length log -> diskGet d (log_addr a) =?= nth a log block0).
+Definition abstr : Abstraction State :=
+  abstraction_compose d.abstr {| abstraction := log_abstraction |}.
+Theorem log_length_ok_nil d b :
+  diskGet d 0 = Some b -> block_to_addr b = 0 -> log_length_ok d nil.
+Proof.
+(unfold log_length_ok; intros).
+(rewrite H; simpl; eauto).
+Qed.
+Theorem log_abstraction_nil d b :
+  diskGet d 0 = Some b -> block_to_addr b = 0 -> log_abstraction d nil.
+Proof.
+(unfold log_abstraction; intros).
+split.
+-
+eauto using log_length_ok_nil.
+-
+(simpl; intuition).
+(exfalso; lia).
+Add Search Blacklist "Raw" "Proofs".
+Set Search Output Name Only.
+Redirect "/var/folders/5x/1mdbpbjd7012l971fq0zkj2w0000gn/T/coqeWX6KU"
+SearchPattern _.
+Remove Search Blacklist "Raw" "Proofs".
+Unset Search Output Name Only.
+Qed.
+Theorem init_ok : init_abstraction init recover abstr inited_any.
+Proof.
+(eapply then_init_compose; eauto).
+step_proc.
+(destruct (lt_dec r 1)).
+-
+step_proc.
+-
+step_proc.
+step_proc.
+step_proc.
+(exists nil; simpl).
+(split; auto).
+(eapply log_abstraction_nil; eauto).
+(autorewrite with upd; auto).
+Qed.
+Theorem get_len_ok :
+  proc_spec
+    (fun (_ : unit) state =>
+     {|
+     pre := True;
+     post := fun r state' => state' = state /\ block_to_addr r = a;
+     recovered := fun _ state' => state' = state |}) get_len d.recover.
+(* Auto-generated comment: Failed. *)
 
